Day 8

problems/8/Problem8.dfy
@@ -1,9 +1,142 @@
+include "../../parser/split.dfy"
+include "../../parser/parseInt.dfy"
 module Problem8 {
+    import opened Split
+    import opened ParseInt
+    import opened Std.Collections.Seq
+
+    method parseInput(input: string) returns (attenas: map<char, seq<(nat, nat)>>,dim: (nat, nat))
+    {
+        attenas := map[];
+        var lines := splitOnBreak(input);
+        expect |lines| > 0;
+        dim := (|lines[0]|, |lines|-1);
+        for i := 0 to |lines| 
+        {
+            if lines[i] != "" {
+                for j := 0 to |lines[i]| 
+                {
+                    if lines[i][j] != '.' {
+                        if lines[i][j] !in attenas {
+                            attenas := attenas[lines[i][j] := [(j, i)]];
+                        }else {
+                            attenas := attenas[lines[i][j] := attenas[lines[i][j]] + [(j, i)]];
+                        }
+                    }
+                }
+            }
+        }
+    }
+
+    function abs(x: int): int
+    {
+        if x < 0 then -x else x
+    }
+
+    function diff(a: (nat, nat), b: (nat, nat)): (int, int)
+    {
+        (a.0 - b.0, a.1 - b.1)
+    }
+
+    function addDiff(a: (nat, nat), b: (int, int)): (int, int)
+    {
+        (a.0 + b.0, a.1 + b.1)
+    }
+
+    function scalarMulDiff(a: (int, int), c: int): (int, int)
+    {
+        (a.0 * c, a.1 * c)
+    }
+
+    function subDiff(a: (nat, nat), b: (int, int)): (int, int)
+    {
+        (a.0 - b.0, a.1 - b.1)
+    }
+
+    predicate InBounds(p: (int, int), dim: (nat, nat)) 
+    {
+        0 <= p.0 < dim.0 && 0 <= p.1 < dim.1
+    }
+
     method problem8_1(input: string) returns (x: int) {
-        return 3;
+        var data, dim := parseInput(input);
+        print dim, "\n";
+        print data, "\n";
+        var antinodes: set<(int, int)> := {};
+        var freqs := data.Keys;
+        var freqSeq := SetToSeq(freqs);
+        assert forall x :: x in multiset(freqSeq) ==> x in freqs;
+        for i := 0 to |freqSeq| 
+        {
+            var freq := freqSeq[i];
+            var freqData := data[freq];
+            for j := 0 to |freqData| 
+            {
+                var a := freqData[j];
+                for k := j+1 to |freqData| 
+                {
+                    var b := freqData[k];
+                    if a != b {
+                        var d := diff(a, b);
+                        var c := addDiff(a, d);
+                        if InBounds(c, dim) {
+                            antinodes := antinodes + {c};
+                        }
+                        var e := subDiff(b, d);
+                        if InBounds(e, dim) {
+                            antinodes := antinodes + {e};
+                        }
+                    }
+                }
+            }
+        }
+        x := |antinodes|;
     }
 
     method problem8_2(input: string) returns (x: int) {
-        return 4;
+        var data, dim := parseInput(input);
+        print dim, "\n";
+        print data, "\n";
+        var antinodes: set<(int, int)> := {};
+        var freqs := data.Keys;
+        var freqSeq := SetToSeq(freqs);
+        assert forall x :: x in multiset(freqSeq) ==> x in freqs;
+        for i := 0 to |freqSeq| 
+        {
+            var freq := freqSeq[i];
+            var freqData := data[freq];
+            for j := 0 to |freqData| 
+            {
+                var a := freqData[j];
+                for k := j+1 to |freqData| 
+                {
+                    var b := freqData[k];
+                    if a != b {
+                        var d := diff(a, b);
+                        assert d != (0, 0);
+                        var c := addDiff(a, d);
+                        ghost var ci := 1;
+                        antinodes := antinodes + {a};
+                        while InBounds(c, dim)
+                            invariant c == addDiff(a, scalarMulDiff(d, ci))
+                            decreases abs(dim.0 - c.0), abs(dim.1 - c.1)
+                        {
+                            antinodes := antinodes + {c};
+                            c := addDiff(c, d);
+                            ci := ci + 1;
+                        }
+                        antinodes := antinodes + {b};
+                        var e := subDiff(b, d);
+                        while InBounds(e, dim)
+                        {
+                            antinodes := antinodes + {e};
+                            e := subDiff(e, d);
+                        }
+                    }
+                }
+            }
+        }
+        x := |antinodes|;
+
     }
 }
